user 3, session 7199, part 483

diffs-w-failures/3/user-3-session-7199.v
@@ -38,6 +38,11 @@ Notation "d [ a |=> bs ]" := (diskUpds d a bs)
   (at level 12, left associativity).
 Set Silent.
 Opaque diskGet.
+Unset Silent.
+Set Diffs "off".
+Set Printing Width 68.
+Set Silent.
+Set Default Goal Selector "!".
 Module Log (d: OneDiskAPI)<: LogAPI.
 Definition len_addr : addr := 0.
 Definition log_addr a : addr := S a.
@@ -45,9 +50,12 @@ Definition init' : proc InitResult :=
   size <- d.size;
   (if lt_dec size 1
    then Ret InitFailed
-   else len0 <- addr_to_block 0; _ <- d.write len_addr len0; Ret Initialized).
+   else
+    len0 <- addr_to_block 0;
+    _ <- d.write len_addr len0; Ret Initialized).
 Definition init := then_init d.init init'.
-Definition get_len : proc addr := b <- d.read len_addr; Ret (block_to_addr b).
+Definition get_len : proc addr :=
+  b <- d.read len_addr; Ret (block_to_addr b).
 Definition get_at (a : addr) : proc block := d.read (log_addr a).
 Fixpoint get_upto (a : addr) : proc (list block) :=
   match a with
@@ -73,29 +81,14 @@ Definition append (bs : list block) : proc bool :=
 Definition reset : proc unit :=
   len0 <- addr_to_block 0; d.write len_addr len0.
 Definition recover : proc unit := d.recover.
-Unset Silent.
-Set Diffs "off".
-Timeout 1 Check @firstn_length.
-Timeout 1 Check @len_addr.
-Timeout 1 Check @len_addr.
-Timeout 1 Check @len_addr.
-Set Printing Width 78.
 Definition log_length_ok (d : disk) (log : list block) :=
-  forall b, diskGet d len_addr =?= b -> block_to_addr b = length log.
-Redirect "/var/folders/5x/1mdbpbjd7012l971fq0zkj2w0000gn/T/coqI1IV5W"
-Print Ltac Signatures.
-Timeout 1 Print Grammar tactic.
-Add Search Blacklist "Raw" "Proofs".
-Set Search Output Name Only.
-Redirect "/var/folders/5x/1mdbpbjd7012l971fq0zkj2w0000gn/T/coqfLWLGq"
-SearchPattern _.
-Remove Search Blacklist "Raw" "Proofs".
-Unset Search Output Name Only.
-Set Silent.
+  forall b,
+  diskGet d len_addr =?= b -> block_to_addr b = length log.
 Definition log_size_ok (d : disk) (log : list block) :=
   diskSize d >= 1 + length log.
 Definition log_contents_ok (d : disk) (log : list block) :=
-  forall a, a < length log -> diskGet d (log_addr a) =?= nth a log block0.
+  forall a,
+  a < length log -> diskGet d (log_addr a) =?= nth a log block0.
 Definition log_abstraction (d : disk) (log : list block) : Prop :=
   log_length_ok d log /\ log_size_ok d log /\ log_contents_ok d log.
 Theorem abstr_length_proj d log :
@@ -103,7 +96,8 @@ Theorem abstr_length_proj d log :
 Proof.
 (unfold log_abstraction; intuition).
 Qed.
-Theorem abstr_size_proj d log : log_abstraction d log -> log_size_ok d log.
+Theorem abstr_size_proj d log :
+  log_abstraction d log -> log_size_ok d log.
 Proof.
 (unfold log_abstraction; intuition).
 Qed.
@@ -112,12 +106,14 @@ Theorem abstr_contents_proj d log :
 Proof.
 (unfold log_abstraction; intuition).
 Qed.
-Hint Resolve abstr_length_proj abstr_size_proj abstr_contents_proj: core.
+Hint Resolve abstr_length_proj abstr_size_proj abstr_contents_proj:
+  core.
 Definition abstr : Abstraction State :=
   abstraction_compose d.abstr {| abstraction := log_abstraction |}.
 Lemma diskGet_eq_values :
   forall d a b b',
-  diskGet d a =?= b -> diskGet d a =?= b' -> a < diskSize d -> b = b'.
+  diskGet d a =?= b ->
+  diskGet d a =?= b' -> a < diskSize d -> b = b'.
 Proof.
 (intros).
 (destruct (diskGet d a) eqn:?; simpl in *).
@@ -133,47 +129,20 @@ Ltac
   | H:diskGet ?d ?a =?= ?b, H':diskGet ?d ?a =?= ?b'
     |- _ =>
         assert (b = b') by
-         (apply (@diskGet_eq_values d a b b'); try lia; auto); subst
+         (apply (@diskGet_eq_values d a b b'); try lia; auto);
+         subst
   end.
-Unset Silent.
-Set Diffs "off".
-Timeout 1 Check @block.
-Timeout 1 Check @log_addr.
-Timeout 1 Check @log_addr.
-Timeout 1 Check @log_addr.
-Timeout 1 Check @block.
-Timeout 1 Check @firstn_length.
-Timeout 1 Check @firstn_length.
-Timeout 1 Check @len_addr.
-Timeout 1 Check @len_addr.
-Timeout 1 Check @len_addr.
-Timeout 1 Check @len_addr.
-Set Printing Width 78.
 Theorem log_length_ok_nil d b :
-  diskGet d len_addr = Some b -> block_to_addr b = 0 -> log_length_ok d nil.
+  diskGet d len_addr = Some b ->
+  block_to_addr b = 0 -> log_length_ok d nil.
 Proof.
 (unfold log_length_ok; intros).
 (rewrite H in *; simpl in *; subst).
 auto.
-Add Search Blacklist "Raw" "Proofs".
-Set Search Output Name Only.
-Redirect "/var/folders/5x/1mdbpbjd7012l971fq0zkj2w0000gn/T/coqH0Mv0e"
-SearchPattern _.
-Remove Search Blacklist "Raw" "Proofs".
-Unset Search Output Name Only.
 Qed.
-Unset Silent.
-Set Diffs "off".
-Timeout 1 Check @firstn_length.
-Timeout 1 Check @firstn_length.
-Timeout 1 Check @len_addr.
-Timeout 1 Check @len_addr.
-Timeout 1 Check @len_addr.
-Set Printing Width 78.
-Set Silent.
-Set Silent.
 Theorem log_abstraction_nil d b :
-  diskGet d len_addr = Some b -> block_to_addr b = 0 -> log_abstraction d nil.
+  diskGet d len_addr = Some b ->
+  block_to_addr b = 0 -> log_abstraction d nil.
 Proof.
 (unfold log_abstraction; intros).
 intuition.
@@ -182,38 +151,18 @@ eauto using log_length_ok_nil.
 -
 (unfold log_size_ok).
 (destruct d; simpl in *; [  | lia ]).
-Unset Silent.
-Set Diffs "off".
-Timeout 1 Check @firstn_length.
-Timeout 1 Check @len_addr.
-Timeout 1 Check @len_addr.
-Timeout 1 Check @len_addr.
-Set Printing Width 78.
-Show.
 (assert (diskGet nil len_addr = None)).
 {
-Set Silent.
 (apply disk_oob_eq).
-Unset Silent.
 (simpl; lia).
 }
 congruence.
 -
 (unfold log_contents_ok; simpl in *; intuition).
 (exfalso; lia).
-Add Search Blacklist "Raw" "Proofs".
-Set Search Output Name Only.
-Redirect "/var/folders/5x/1mdbpbjd7012l971fq0zkj2w0000gn/T/coqRmv5ZP"
-SearchPattern _.
-Remove Search Blacklist "Raw" "Proofs".
-Unset Search Output Name Only.
 Qed.
-Set Silent.
-Set Silent.
 Theorem init_ok : init_abstraction init recover abstr inited_any.
-Unset Silent.
 Proof.
-Set Silent.
 (eapply then_init_compose; eauto).
 step_proc.
 (destruct (lt_dec r 1)).
@@ -226,32 +175,9 @@ step_proc.
 (exists nil; simpl).
 (split; auto).
 (eapply log_abstraction_nil; eauto).
-Unset Silent.
-Set Diffs "off".
-Set Printing Width 78.
-Show.
-Unset Silent.
-Set Diffs "off".
-Timeout 1 Check @Ascii.nat_ascii_bounded.
-Timeout 1 Check @Wf.F_unfold.
-Timeout 1 Check @firstn_length.
-Timeout 1 Check @firstn_length.
-Timeout 1 Check @len_addr.
-Timeout 1 Check @len_addr.
-Timeout 1 Check @len_addr.
-Timeout 1 Check @len_addr.
-Set Printing Width 78.
-Show.
 (unfold len_addr).
 (autorewrite with upd; auto).
-Add Search Blacklist "Raw" "Proofs".
-Set Search Output Name Only.
-Redirect "/var/folders/5x/1mdbpbjd7012l971fq0zkj2w0000gn/T/coqGXgs2S"
-SearchPattern _.
-Remove Search Blacklist "Raw" "Proofs".
-Unset Search Output Name Only.
 Qed.
-Set Silent.
 Theorem log_abstraction_length d bs :
   log_abstraction d bs -> log_length_ok d bs.
 Proof.
@@ -275,7 +201,8 @@ Theorem get_len_ok :
      {|
      pre := log_length_ok state bs /\ log_size_ok state bs;
      post := fun r state' => state' = state /\ r = length bs;
-     recovered := fun _ state' => state' = state |}) get_len recover d.abstr.
+     recovered := fun _ state' => state' = state |}) get_len
+    recover d.abstr.
 Proof.
 (unfold get_len; intros).
 step_proc.
@@ -289,7 +216,8 @@ Theorem get_len_abstr_ok :
      {|
      pre := True;
      post := fun r state' => state' = state /\ r = length state;
-     recovered := fun _ state' => state' = state |}) get_len recover abstr.
+     recovered := fun _ state' => state' = state |}) get_len
+    recover abstr.
 Proof.
 (apply spec_abstraction_compose).
 (eapply proc_spec_weaken; eauto).
@@ -309,7 +237,8 @@ Theorem get_at_ok a :
     (fun (_ : unit) state =>
      {|
      pre := a < length state;
-     post := fun r state' => state' = state /\ nth a state block0 = r;
+     post := fun r state' =>
+             state' = state /\ nth a state block0 = r;
      recovered := fun _ state' => state' = state |}) 
     (get_at a) recover abstr.
 Proof.
@@ -325,375 +254,3 @@ Proof.
 (pose proof (H3 a); intuition).
 (assert (v = nth a bs block0)).
 (eapply diskGet_eq_values; eauto).
-auto.
-Qed.
-Hint Resolve get_at_ok: core.
-Theorem recover_wipe : rec_wipe recover abstr no_wipe.
-Proof.
-(unfold rec_wipe; simpl; intros).
-(apply spec_abstraction_compose).
-step_proc.
-(destruct a as [_ bs]; simpl in *; intuition eauto).
-Qed.
-Hint Resolve recover_wipe: core.
-Lemma firstn_one_more :
-  forall (a : nat) (d : list block),
-  S a <= length d -> firstn a d ++ [nth a d block0] = firstn (S a) d.
-Proof.
-(intros).
-generalize dependent a.
-(induction d; simpl; intros).
--
-(exfalso; lia).
--
-(destruct a0; simpl in *; auto).
-(rewrite IHd by lia; auto).
-Qed.
-Opaque firstn.
-Theorem get_upto_ok a :
-  proc_spec
-    (fun (_ : unit) state =>
-     {|
-     pre := a <= length state;
-     post := fun r state' => state' = state /\ r = firstn a state;
-     recovered := fun _ state' => state' = state |}) 
-    (get_upto a) recover abstr.
-Proof.
-(induction a; simpl).
--
-step_proc.
--
-step_proc.
-step_proc.
-intuition eauto.
-{
-lia.
-}
-step_proc.
-auto using firstn_one_more.
-Qed.
-Hint Resolve get_upto_ok: core.
-Theorem get_ok : proc_spec get_spec get recover abstr.
-Proof.
-(unfold get, get_spec; intros).
-step_proc.
-(eapply proc_spec_weaken; eauto).
-(unfold spec_impl; simpl; intuition).
-(descend; intuition eauto).
-(rewrite firstn_all; auto).
-Qed.
-Unset Silent.
-Set Diffs "off".
-Set Printing Width 78.
-Set Silent.
-Theorem log_contents_ok_unchanged d bs a0 b :
-  log_size_ok d bs ->
-  log_contents_ok d bs ->
-  a0 >= length bs -> log_contents_ok (diskUpd d (log_addr a0) b) bs.
-Proof.
-(unfold log_size_ok, log_contents_ok; intros).
-(destruct (a == a0); subst; autorewrite with upd; auto).
-(simpl; auto).
-Qed.
-Theorem log_size_ok_shrink d bs bs' :
-  log_size_ok d (bs ++ bs') -> log_size_ok d bs.
-Proof.
-(unfold log_size_ok; simpl).
-(rewrite app_length; intros).
-lia.
-Qed.
-Hint Resolve log_size_ok_shrink: core.
-Hint Rewrite app_length : list.
-Theorem log_contents_ok_prefix d bs bs' :
-  log_contents_ok d (bs ++ bs') -> log_contents_ok d bs.
-Proof.
-(unfold log_contents_ok; intros).
-specialize (H a).
-(rewrite app_nth1 in H by lia).
-(apply H).
-(rewrite app_length; lia).
-Qed.
-Hint Resolve log_contents_ok_prefix: core.
-Theorem log_contents_ok_append d bs b bs' :
-  log_size_ok d (bs ++ b :: bs') ->
-  log_contents_ok d bs ->
-  log_contents_ok (diskUpd d (log_addr (length bs)) b) (bs ++ [b]).
-Proof.
-(unfold log_contents_ok; intros).
-(assert (log_addr (length bs) < diskSize d)).
-{
-(unfold log_size_ok, log_addr, diskSize in *).
-(rewrite app_length in *; simpl in *).
-lia.
-}
-(destruct (a == length bs); subst; autorewrite with upd).
--
-(simpl).
-(rewrite app_nth2 by lia).
-replace (length bs - length bs) with 0 by lia.
-reflexivity.
--
-(assert (a < length bs)).
-{
-(rewrite app_length in *; simpl in *; lia).
-}
-(rewrite app_nth1 by lia).
-auto.
-Qed.
-Hint Resolve log_contents_ok_append: core.
-Theorem append_at_ok a bs' :
-  proc_spec
-    (fun (bs : list block) state =>
-     {|
-     pre := a = length bs /\
-            log_size_ok state (bs ++ bs') /\ log_contents_ok state bs;
-     post := fun r state' =>
-             diskGet state' len_addr = diskGet state len_addr /\
-             diskSize state' = diskSize state /\
-             log_size_ok state' (bs ++ bs') /\
-             log_contents_ok state' (bs ++ bs');
-     recovered := fun _ state' =>
-                  diskGet state' len_addr = diskGet state len_addr /\
-                  diskSize state' = diskSize state /\
-                  log_contents_ok state' bs |}) (append_at a bs') recover
-    d.abstr.
-Proof.
-generalize dependent a.
-(induction bs'; simpl; intros).
--
-step_proc.
-intuition eauto.
-(rewrite app_nil_r; auto).
--
-step_proc.
-(intuition eauto; autorewrite with upd; auto).
-(eapply proc_spec_weaken; eauto).
-(unfold spec_impl; simpl; intuition).
-(exists (a' ++ [a]); intuition eauto; autorewrite with upd list in *; eauto).
-+
-(simpl; lia).
-+
-(unfold log_size_ok in *; simpl in *).
-autorewrite with upd list in *.
-(simpl in *; lia).
-+
-(unfold log_size_ok in *; simpl in *).
-autorewrite with upd list in *.
-(simpl in *; lia).
-+
-(rewrite <- app_assoc in *; simpl in *; auto).
-Qed.
-Hint Resolve append_at_ok: core.
-Theorem log_abstraction_preserved d bs d' :
-  log_abstraction d bs ->
-  diskGet d' len_addr = diskGet d len_addr ->
-  diskSize d' = diskSize d -> log_contents_ok d' bs -> log_abstraction d' bs.
-Proof.
-(unfold log_abstraction, log_length_ok, log_size_ok; intuition).
--
-replace (diskGet d' len_addr) in *.
-auto.
--
-congruence.
-Qed.
-Theorem abstr_length_sz_bound d bs :
-  log_size_ok d bs -> len_addr < diskSize d.
-Proof.
-(unfold log_size_ok, len_addr, diskSize).
-(intros; lia).
-Qed.
-Unset Silent.
-Hint Resolve abstr_length_sz_bound: core.
-Timeout 1 Check @log_contents_ok.
-Timeout 1 Check @log_length_ok.
-Timeout 1 Check @log_contents_ok.
-Timeout 1 Check @log_contents_ok.
-Timeout 1 Check @log_length_ok.
-Timeout 1 Check @log_length_ok.
-Timeout 1 Check @firstn_length.
-Timeout 1 Check @firstn_length.
-Timeout 1 Check @len_addr.
-Timeout 1 Check @len_addr.
-Timeout 1 Check @len_addr.
-Theorem log_contents_ok_len_change d bs b :
-  log_size_ok d bs ->
-  log_contents_ok d bs -> log_contents_ok (diskUpd d len_addr b) bs.
-Proof.
-Unset Silent.
-Set Diffs "off".
-Timeout 1 Check @firstn_length.
-Timeout 1 Check @firstn_length.
-Timeout 1 Check @len_addr.
-Timeout 1 Check @len_addr.
-Timeout 1 Check @len_addr.
-Timeout 1 Check @len_addr.
-Set Printing Width 78.
-Show.
-(unfold log_size_ok, log_contents_ok, len_addr; intros).
-Timeout 1 Check @Ascii.nat_ascii_bounded.
-Timeout 1 Check @log_contents_ok.
-Timeout 1 Check @log_contents_ok.
-Timeout 1 Check @log_addr.
-Timeout 1 Check @log_addr.
-Timeout 1 Check @log_addr.
-Timeout 1 Check @Byte.xa0.
-Timeout 1 Check @spec_abstraction_compose.
-Timeout 1 Check @split.
-Unset Silent.
-Set Diffs "off".
-Set Printing Width 78.
-Show.
-Unset Silent.
-Set Diffs "off".
-Timeout 1 Check @rec_wipe_compose.
-Timeout 1 Check @nodup.
-Set Printing Width 78.
-Show.
-(destruct (0 == log_addr a); autorewrite with upd).
--
-(exfalso; unfold log_addr in *; lia).
--
-Timeout 1 Check @Tauto.A.
-auto.
-Add Search Blacklist "Raw" "Proofs".
-Set Search Output Name Only.
-Redirect "/var/folders/5x/1mdbpbjd7012l971fq0zkj2w0000gn/T/coqIydDso"
-SearchPattern _.
-Remove Search Blacklist "Raw" "Proofs".
-Unset Search Output Name Only.
-Qed.
-Set Silent.
-Lemma log_abstraction_commit :
-  forall bs bs' : list block,
-  forall d' : State,
-  log_size_ok d' (bs ++ bs') ->
-  log_contents_ok d' (bs ++ bs') ->
-  forall len_b : block,
-  block_to_addr len_b = length bs + length bs' ->
-  log_abstraction (diskUpd d' len_addr len_b) (bs ++ bs').
-Proof.
-(intros).
-(assert (len_addr < diskSize d') by eauto).
-(unfold log_abstraction; intuition).
--
-(unfold log_length_ok in *; intros; autorewrite with upd list in *).
-(simpl in *; intuition).
--
-(unfold log_size_ok in *; autorewrite with upd list in *).
-Unset Silent.
-lia.
--
-Timeout 1 Check @app.
-Timeout 1 Check @app.
-Timeout 1 Check @incl_appl.
-Timeout 1 Check @log_contents_ok.
-Timeout 1 Check @log_contents_ok.
-Timeout 1 Check @log_contents_ok.
-Timeout 1 Check @log_contents_ok.
-Timeout 1 Check @log_contents_ok_append.
-Timeout 1 Check @log_contents_ok_append.
-Timeout 1 Check @log_contents_ok_append.
-Unset Silent.
-Set Diffs "off".
-Timeout 1 Check @Tauto.A.
-Set Printing Width 78.
-Show.
-(apply log_contents_ok_len_change; auto).
-Add Search Blacklist "Raw" "Proofs".
-Set Search Output Name Only.
-Redirect "/var/folders/5x/1mdbpbjd7012l971fq0zkj2w0000gn/T/coqkTH0AK"
-SearchPattern _.
-Remove Search Blacklist "Raw" "Proofs".
-Unset Search Output Name Only.
-Qed.
-Hint Resolve log_abstraction_commit: core.
-Set Silent.
-Theorem log_length_ok_unchanged d bs d' :
-  log_length_ok d bs ->
-  diskGet d' len_addr = diskGet d len_addr -> log_length_ok d' bs.
-Proof.
-(unfold log_length_ok; intros).
-(rewrite H0 in *).
-eauto.
-Qed.
-Hint Resolve log_length_ok_unchanged: core.
-Theorem append_ok :
-  forall v, proc_spec (append_spec v) (append v) recover abstr.
-Proof.
-(unfold append; intros).
-(apply spec_abstraction_compose).
-step_proc.
-(destruct a' as [[] bs]; simpl in *).
-intuition eauto.
-step_proc.
-(descend; intuition eauto).
-destruct matches.
--
-step_proc.
-(descend; intuition eauto).
-{
-(unfold log_size_ok; autorewrite with list; auto).
-}
-{
-(exists bs; intuition eauto using log_abstraction_preserved).
-}
-step_proc.
-intuition.
-{
-(exists bs; eauto using log_abstraction_preserved).
-}
-step_proc.
-intuition.
-{
-(exists bs; intuition eauto).
-(unfold log_abstraction; intuition eauto).
-}
-{
-Unset Silent.
-(exists (bs ++ v); intuition).
-}
-step_proc.
-intuition.
-{
-(descend; intuition eauto).
-}
-{
-(descend; intuition eauto).
-}
--
-step_proc.
-intuition eauto.
-Add Search Blacklist "Raw" "Proofs".
-Set Search Output Name Only.
-Redirect "/var/folders/5x/1mdbpbjd7012l971fq0zkj2w0000gn/T/coqddJgaw"
-SearchPattern _.
-Remove Search Blacklist "Raw" "Proofs".
-Unset Search Output Name Only.
-Qed.
-Theorem reset_ok : proc_spec reset_spec reset recover abstr.
-Set Silent.
-Proof.
-(unfold reset; intros).
-(apply spec_abstraction_compose).
-step_proc.
-(destruct a' as [[] bs]; simpl in *).
-intuition.
-{
-(descend; intuition eauto).
-}
-(eapply proc_spec_weaken; eauto).
-(unfold spec_impl; simpl; intuition).
-(descend; intuition eauto).
-{
-(descend; intuition eauto).
-(eapply log_abstraction_nil; eauto).
-(rewrite diskUpd_eq; eauto).
-}
-{
-(descend; intuition eauto).
-(eapply log_abstraction_nil; eauto).
-(rewrite diskUpd_eq; eauto).
-}
-Qed.
-Unset Silent.
-End Log.
